<section xml:id="sec_functions_hints">
  <title>Hints for
  <q>Functions: basic concepts</q>
  exercises</title>
  <p>
    <xref ref="exercise_functions_funtable">Exercise</xref>(e): There is a formula of the form <m>f(x) = ax^2 + bx + c</m>
  </p>
  <p>
    <xref ref="exercise_functions_45">Exercise</xref>: Can there be any elements in the codomain that are not in the range?.
  </p>
  <p>
    <xref ref="exercise_functions_NxNBijection">Exercise</xref>(a): Consider the values <m>f(1,i)</m> for
    <m>i=1,2,3,\ldots</m>. (b): Consider the values <m>f(2,j)</m> and <m>f(1,i)</m>.
  </p>
  <p>
    <xref ref="exercise_functions_NxN">Exercise</xref>(a): Given any element <m>(i,j)</m> of <m>\mathbb{Z} \times \mathbb{Z}</m>,
    set <m>i=m+n</m> and <m>j=m+2n</m> and solve for <m>m</m> and <m>n</m> in terms of <m>i</m> and <m>j</m>.
  </p>
  <p>
    <xref ref="exercise_functions_NxN">Exercise</xref>(b): Suppose that <m>g(m,n) = g(p,q)</m>.
    It follows that <m>(m + n, m + 2n) = (p + q, p + 2q)</m>.
  </p>
  <p>
    <xref ref="exercise_functions_BijectionComposeExer">Exercise</xref>: (a) You only need to show that
    <m>g \compose f</m> is both one-to-one and onto.
    Use the previous exercises. (b) Prove by contradiction.
    Suppose that there exists a <m>y</m> such that <m>g_1(y) \neq g_2(y)</m>.
    Then what can you say about
    <m>f \compose g_1(y)</m> and <m>f \compose g_2(y)</m>?
  </p>
  <p>
    <xref ref="exercise_functions_inverMod">Exercise</xref>: (c) Use <xref ref="proposition_modular_mod_eq_solution">Proposition</xref>,
    and recall that <m>ax \equiv 1 \pmod{n}</m> means the same thing as
    <m>a \odot x = 1</m> for <m>a,x \in \mathbb{Z}_n</m>.
    You may use this fact to find an inverse for <m>f_a</m>. (d) Use the fact that
    <m>a \odot x = 1</m> has no solution to show that <m>f_a</m> is not onto,
    which implies that <m>f_a</m> has no inverse.
  </p>
  <p>
    <xref ref="exercise_functions_IdAInverse">Exercise</xref>: (a) Notice that <m>f(x)=x</m> is the identify function when the set <m>A</m> is equal to <m>\mathbb{R}</m>.
    Think about how you would show that <m>f(x)</m> is invertible in this case.
    Then apply the same proof,
    replacing <m>x</m> with <m>a</m> and <m>f</m> with <m>Id_A</m>. (b) Again,
    think of the case <m>f(x)=x</m>.
    What is the inverse of this function?
  </p>
  <p>
    <xref ref="exercise_functions_InverseBijection2">Exercise</xref>: Given that <m>f</m> is a bijection from <m>X</m> to <m>Y</m>.
    We may define a function <m>g</m> from <m>Y</m> to <m>X</m> as follows.
    Given any <m>y \in Y</m>,
    since <m>f</m> is onto there is at least one <m>x</m> such that <m>f(x) = y</m>.
    Furthermore,
    since <m>f</m> is one-to-one there is at most one <m>x</m> such that <m>f(x)=y</m>.
    Putting these two facts together gives us that there is <em>exactly</em>
    one <m>x</m> such that <m>f(x)=y</m>.
    We may define <m>g(y)</m> as this unique <m>x</m>.
    It remains to show that for any <m>y \in Y</m>, <m>f(g(y))=y</m>;
    and for any <m>x \in X</m>, <m>g(f(x))=x</m>.
  </p>
  <p>
    <xref ref="exercise_functions_InverseIdentityExers">Exercise</xref>: (a) Apply <xref ref="def_invfna">Definition</xref> directly,
    replacing <m>f</m> with <m>g \circ f</m> and <m>g</m> with
    <m>g^{-1} \circ f^{-1}</m>. (b) Apply <xref ref="def_invfna">Definition</xref> again,
    this time replacing <m>f</m> with <m>f^{-1}</m>.
    What should <m>g</m> be replaced with?
  </p>
</section>